Add algebraic effects for locals and loops

theories/Imperative.v
@@ -8,37 +8,83 @@ Record Environment := { arrayType: string -> Type; arrays: forall (name : string
 
 Record Locals := { numbers: string -> Z; booleans: string -> bool }.
 
-Inductive Action (arrayType : string -> Type) (effectType : Type) (effectResponse : effectType -> Type) (returnType : Type) :=
+Inductive Action (effectType : Type) (effectResponse : effectType -> Type) (returnType : Type) :=
 | Done (returnValue : returnType)
-| Dispatch (effect : effectType) (continuation : effectResponse effect -> Action arrayType effectType effectResponse returnType).
+| Dispatch (effect : effectType) (continuation : effectResponse effect -> Action effectType effectResponse returnType).
 
-Fixpoint bind {arrayType effectType effectResponse A B} (a : Action arrayType effectType effectResponse A) (f : A -> Action arrayType effectType effectResponse B) : Action arrayType effectType effectResponse B :=
+Fixpoint bind {effectType effectResponse A B} (a : Action effectType effectResponse A) (f : A -> Action effectType effectResponse B) : Action effectType effectResponse B :=
   match a with
-  | Done _ _ _ _ value => f value
-  | Dispatch _ _ _ _ effect continuation => Dispatch _ _ _ _ effect (fun response => bind (continuation response) f)
+  | Done _ _ _ value => f value
+  | Dispatch _ _ _ effect continuation => Dispatch _ _ _ effect (fun response => bind (continuation response) f)
   end.
 
-Lemma leftIdentity {arrayType effectType effectResponse A B} (x : A) (f : A -> Action arrayType effectType effectResponse B) : bind (Done _ _ _ _ x) f = f x.
+Lemma leftIdentity {effectType effectResponse A B} (x : A) (f : A -> Action effectType effectResponse B) : bind (Done _ _ _ x) f = f x.
 Proof. easy. Qed.
 
-Lemma rightIdentity {arrayType effectType effectResponse A} (x : Action arrayType effectType effectResponse A) : bind x (Done _ _ _ _) = x.
+Lemma rightIdentity {effectType effectResponse A} (x : Action effectType effectResponse A) : bind x (Done _ _ _) = x.
 Proof.
-  pose proof (ltac:(intros T next h; now apply functional_extensionality): forall T next, (forall x, bind (next x) (Done arrayType effectType effectResponse A) = next x) -> (fun (x : T) => bind (next x) (Done arrayType effectType effectResponse A)) = next) as H.
+  pose proof (ltac:(intros T next h; now apply functional_extensionality): forall T next, (forall x, bind (next x) (Done effectType effectResponse A) = next x) -> (fun (x : T) => bind (next x) (Done effectType effectResponse A)) = next) as H.
   induction x as [| a next IH]; try easy; simpl; now (rewrite (H _ _ IH) || rewrite IH).
 Qed.
 
-Lemma assoc {arrayType effectType effectResponse A B C} (x : Action arrayType effectType effectResponse A) (f : A -> Action arrayType effectType effectResponse B) (g : B -> Action arrayType effectType effectResponse C) : bind x (fun x => bind (f x) g) = bind (bind x f) g.
+Lemma assoc {effectType effectResponse A B C} (x : Action effectType effectResponse A) (f : A -> Action effectType effectResponse B) (g : B -> Action effectType effectResponse C) : bind x (fun x => bind (f x) g) = bind (bind x f) g.
 Proof.
   pose proof (ltac:(intros T next h; now apply functional_extensionality): forall T next, (forall x, bind (next x) (fun x => bind (f x) g) = bind (bind (next x) f) g) -> (fun (x : T) => bind (next x) (fun x => bind (f x) g)) = (fun x => bind (bind (next x) f) g)) as H.
   induction x as [| a next IH]; try easy; simpl; now (rewrite IH || rewrite (H _ _ IH)).
 Qed.
 
-Definition shortCircuitAnd arrayType effectType effectResponse (a b : Action arrayType effectType effectResponse bool) := bind a (fun x => match x with
-  | false => Done _ _ _ _ false
+Definition shortCircuitAnd effectType effectResponse (a b : Action effectType effectResponse bool) := bind a (fun x => match x with
+  | false => Done _ _ _ false
   | true => b
   end).
 
-Definition shortCircuitOr arrayType effectType effectResponse (a b : Action arrayType effectType effectResponse bool) := bind a (fun x => match x with
-  | true => Done _ _ _ _ true
+Definition shortCircuitOr effectType effectResponse (a b : Action effectType effectResponse bool) := bind a (fun x => match x with
+  | true => Done _ _ _ true
   | false => b
   end).
+
+Inductive BasicEffects (arrayType : string -> Type) :=
+| Trap
+| Flush
+| ReadChar
+| WriteChar (value : Z)
+| Retrieve (arrayName : string) (index : Z)
+| Store (arrayName : string) (index : Z) (value : arrayType arrayName).
+
+Definition basicEffectsReturnValue {arrayType} (effect : BasicEffects arrayType) : Type :=
+  match effect with
+  | Trap _ => unit
+  | Flush _ => unit
+  | ReadChar _ => Z
+  | WriteChar _ _ => unit
+  | Retrieve _ arrayName _ => arrayType arrayName
+  | Store _ _ _ _ => unit
+  end.
+
+Inductive WithLocalVariables (arrayType : string -> Type) :=
+| BasicEffect (effect : BasicEffects arrayType)
+| BooleanLocalGet (name : string)
+| BooleanLocalSet (name : string) (value : bool)
+| NumberLocalGet (name : string)
+| NumberLocalSet (name : string) (value : Z).
+
+Definition withLocalVariablesReturnValue {arrayType} (effect : WithLocalVariables arrayType) : Type :=
+  match effect with
+  | BasicEffect _ effect => basicEffectsReturnValue effect
+  | BooleanLocalGet _ _ => bool
+  | BooleanLocalSet _ _ _ => unit
+  | NumberLocalGet _ _ => Z
+  | NumberLocalSet _ _ _ => unit
+  end.
+
+Inductive WithLoopControl (arrayType : string -> Type) :=
+| WithLocalVariablesEffect (effect : WithLocalVariables arrayType)
+| Continue
+| Break.
+
+Definition withLoopControlReturnValue {arrayType} (effect : WithLoopControl arrayType) : Type :=
+  match effect with
+  | WithLocalVariablesEffect _ effect => withLocalVariablesReturnValue effect
+  | Continue _ => unit
+  | Break _ => unit
+  end.
